Db.lean
@@ -2,6 +2,7 @@ import Db.Backends.Sql
 import Db.Backends.PostgreSQL.Interpretation
 import Db.Interpretation.Basic
 import Db.Query.Basic
+import Db.Query.DSL
 import Db.Utils.VarChar
 import Db.Migration.Basic
 import Db.Migration.Recipe
